src/Semantics.v
@@ -150,17 +150,18 @@ Section Transition.
     | l :: ll' => (extLabel sys (getLabel l)) ::> (behaviorOf sys ll')
     end.
 
-  Inductive Behavior {SysT StateT LabelT} `{IsSystem SysT StateT} `{HasLabel LabelT}
+  Inductive Behavior {SysT StateT LabelT}
+            `{IsSystem SysT} `{HasInit StateT} `{HasLabel LabelT}
             (ss: Steps SysT StateT LabelT) : SysT -> Trace -> Prop :=
   | Behv: forall sys ll st,
-      ss sys (initsOf sys) ll st ->
+      ss sys initsOf ll st ->
       forall tr,
         tr = behaviorOf sys ll ->
         Behavior ss sys tr.
 
   Definition Refines {SysI SysS StateI LabelI StateS LabelS}
-             `{IsSystem SysI StateI} `{HasLabel LabelI}
-             `{IsSystem SysS StateS} `{HasLabel LabelS}
+             `{IsSystem SysI} `{HasInit StateI} `{HasLabel LabelI}
+             `{IsSystem SysS} `{HasInit StateS} `{HasLabel LabelS}
              (ssI: Steps SysI StateI LabelI) (ssS: Steps SysS StateS LabelS)
              (p: Label -> Label) (impl: SysI) (spec: SysS) :=
     forall ll, Behavior ssI impl ll ->
@@ -183,13 +184,12 @@ Section BState.
       mst_msgs: MessagePool MsgT
     }.
 
-  Definition getBStateInit {MsgT} (sys: System): BState MsgT :=
-    {| mst_oss := initsOf sys;
+  Definition getBStateInit {MsgT}: BState MsgT :=
+    {| mst_oss := initsOf;
        mst_msgs := nil |}.
 
-  Global Instance System_BState_IsSystem {MsgT} : IsSystem System (BState MsgT) :=
-    {| indicesOf := sys_inds;
-       initsOf := getBStateInit |}.
+  Global Instance BState_HasInit {MsgT}: HasInit (BState MsgT) :=
+    {| initsOf := getBStateInit |}.
 
 End BState.
 
@@ -294,14 +294,13 @@ Section TState.
       tst_tid: TrsId
     }.
 
-  Definition getTStateInit (sys: System): TState :=
-    {| tst_oss := initsOf sys;
+  Definition getTStateInit: TState :=
+    {| tst_oss := initsOf;
        tst_msgs := nil;
        tst_tid := trsIdInit |}.
 
-  Global Instance System_TState_IsSystem: IsSystem System TState :=
-    {| indicesOf := sys_inds;
-       initsOf := getTStateInit |}.
+  Global Instance TState_HasInit: HasInit TState :=
+    {| initsOf := getTStateInit |}.
 
 End TState.
 
