src/Simulation.v
@@ -5,8 +5,8 @@ Set Implicit Arguments.
 
 Section Simulation.
   Context {SysI SysS StateI LabelI StateS LabelS: Type}
-          `{IsSystem SysI StateI} `{HasLabel LabelI}
-          `{IsSystem SysS StateS} `{HasLabel LabelS}.
+          `{IsSystem SysI} `{HasInit StateI} `{HasLabel LabelI}
+          `{IsSystem SysS} `{HasInit StateS} `{HasLabel LabelS}.
   Variables (stepI: Step SysI StateI LabelI) (stepS: Step SysS StateS LabelS)
             (sim: StateI -> StateS -> Prop)
             (p: Label -> Label).
@@ -20,17 +20,17 @@ Section Simulation.
       ist1 ≈ sst1 ->
       forall ilbl ist2,
         stepI impl ist1 ilbl ist2 ->
-        match extLabel (StateT:= StateI) impl (getLabel ilbl) with
+        match extLabel impl (getLabel ilbl) with
         | None =>
           (exists sst2 slbl,
               stepS spec sst1 slbl sst2 /\
-              extLabel (StateT:= StateS) spec (getLabel slbl) = None /\
+              extLabel spec (getLabel slbl) = None /\
               ist2 ≈ sst2) \/
           ist2 ≈ sst1
         | Some elbl =>
           (exists sst2 slbl,
               stepS spec sst1 slbl sst2 /\
-              extLabel (StateT:= StateS) spec (getLabel slbl) = Some (p elbl) /\
+              extLabel spec (getLabel slbl) = Some (p elbl) /\
               ist2 ≈ sst2)
         end.
 
@@ -43,42 +43,42 @@ Section Simulation.
         steps stepI impl ist1 ihst ist2 ->
         exists sst2 shst,
           steps stepS spec sst1 shst sst2 /\
-          map p (behaviorOf (StateT:= StateI) impl ihst) =
-          behaviorOf (StateT:= StateS) spec shst /\
+          map p (behaviorOf impl ihst) =
+          behaviorOf spec shst /\
           ist2 ≈ sst2.
   Proof.
     induction 2; simpl; intros;
       [exists sst1, nil; repeat split; auto; constructor|].
 
-    specialize (IHsteps H3).
+    specialize (IHsteps H5).
     destruct IHsteps as [sst2 [shst [? [? ?]]]].
 
-    eapply Hsim in H5; [|exact H8].
+    eapply Hsim in H7; [|exact H10].
     remember (extLabel impl (getLabel lbl)) as ilbl; clear Heqilbl.
     destruct ilbl as [elbl|].
 
-    - destruct H5 as [sst3 [slbl [? [? ?]]]].
+    - destruct H7 as [sst3 [slbl [? [? ?]]]].
       eexists; eexists (_ :: _); repeat split; eauto.
       + econstructor; eauto.
-      + simpl; erewrite H7, H9; simpl.
+      + simpl; erewrite H9, H11; simpl.
         reflexivity.
-    - destruct H5.
-      * destruct H5 as [sst3 [slbl [? [? ?]]]].
+    - destruct H7.
+      * destruct H7 as [sst3 [slbl [? [? ?]]]].
         eexists; eexists (slbl :: _); repeat split; eauto.
         -- econstructor; eauto.
-        -- simpl; rewrite H7, H9; simpl; reflexivity.
+        -- simpl; rewrite H9, H11; simpl; reflexivity.
       * exists sst2, shst; repeat split; auto.
   Qed.
 
-  Hypothesis (Hsimi: sim (initsOf impl) (initsOf spec)).
+  Hypothesis (Hsimi: sim initsOf initsOf).
 
   Theorem simulation_implies_refinement:
     (steps stepI) # (steps stepS) |-- impl ⊑[p] spec.
   Proof.
     unfold Simulates, Refines; intros.
-    inv H3.
-    eapply simulation_steps in H4; [|exact Hsimi].
-    destruct H4 as [sst2 [shst [? [? ?]]]].
+    inv H5.
+    eapply simulation_steps in H6; [|exact Hsimi].
+    destruct H6 as [sst2 [shst [? [? ?]]]].
     econstructor; eauto.
   Qed.
 
@@ -86,8 +86,8 @@ End Simulation.
 
 Section InvSim.
   Context {SysI SysS StateI LabelI StateS LabelS: Type}
-          `{IsSystem SysI StateI} `{HasLabel LabelI}
-          `{IsSystem SysS StateS} `{HasLabel LabelS}.
+          `{IsSystem SysI} `{HasInit StateI} `{HasLabel LabelI}
+          `{IsSystem SysS} `{HasInit StateS} `{HasLabel LabelS}.
   Variables (stepI: Step SysI StateI LabelI) (stepS: Step SysS StateS LabelS)
             (ginv: StateI -> Prop)
             (sim: StateI -> StateS -> Prop)
@@ -105,17 +105,17 @@ Section InvSim.
       forall ilbl ist2,
         linv ilbl ->
         stepI impl ist1 ilbl ist2 ->
-        match extLabel (StateT:= StateI) impl (getLabel ilbl) with
+        match extLabel impl (getLabel ilbl) with
         | None =>
           (exists sst2 slbl,
               stepS spec sst1 slbl sst2 /\
-              extLabel (StateT:= StateS) spec (getLabel slbl) = None /\
+              extLabel spec (getLabel slbl) = None /\
               ist2 ≈ sst2) \/
           ist2 ≈ sst1
         | Some elbl =>
           (exists sst2 slbl,
               stepS spec sst1 slbl sst2 /\
-              extLabel (StateT:= StateS) spec (getLabel slbl) = Some (p elbl) /\
+              extLabel spec (getLabel slbl) = Some (p elbl) /\
               ist2 ≈ sst2)
         end.
 
@@ -131,33 +131,33 @@ Section InvSim.
         steps stepI impl ist1 ihst ist2 ->
         exists sst2 shst,
           steps stepS spec sst1 shst sst2 /\
-          map p (behaviorOf (StateT:= StateI) impl ihst) =
-          behaviorOf (StateT:= StateS) spec shst /\
+          map p (behaviorOf impl ihst) =
+          behaviorOf spec shst /\
           ist2 ≈ sst2.
   Proof.
     induction 4; simpl; intros;
       [exists sst1, nil; repeat split; auto; constructor|].
 
-    inv H5.
-    specialize (IHsteps H3 H4 H11).
+    inv H7.
+    specialize (IHsteps H5 H6 H13).
     destruct IHsteps as [sst2 [shst [? [? ?]]]].
 
-    eapply Hsim in H7;
-      [|exact H9|eapply inv_steps; eauto|exact H10].
+    eapply Hsim in H9;
+      [|exact H11|eapply inv_steps; eauto|exact H12].
     
     remember (extLabel impl (getLabel lbl)) as ilbl; clear Heqilbl.
     destruct ilbl as [elbl|].
 
-    - destruct H7 as [sst3 [slbl [? [? ?]]]].
+    - destruct H9 as [sst3 [slbl [? [? ?]]]].
       eexists; eexists (_ :: _); repeat split; eauto.
       + econstructor; eauto.
-      + simpl; erewrite H8, H12; simpl.
+      + simpl; erewrite H10, H14; simpl.
         reflexivity.
-    - destruct H7.
-      * destruct H7 as [sst3 [slbl [? [? ?]]]].
+    - destruct H9.
+      * destruct H9 as [sst3 [slbl [? [? ?]]]].
         eexists; eexists (slbl :: _); repeat split; eauto.
         -- econstructor; eauto.
-        -- simpl; rewrite H8, H12; simpl; reflexivity.
+        -- simpl; rewrite H10, H14; simpl; reflexivity.
       * exists sst2, shst; repeat split; auto.
   Qed.
 
